theories/LogicalRelation/Reflexivity.v
@@ -1,50 +1,40 @@
 (** * LogRel.LogicalRelation.Reflexivity: reflexivity of the logical relation. *)
 Require Import PeanoNat.
 From LogRel.AutoSubst Require Import core unscoped Ast Extra.
-From LogRel Require Import Utils BasicAst LContexts Context NormalForms Weakening GenericTyping LogicalRelation DeclarativeInstance.
+From LogRel Require Import Utils BasicAst LContexts Context NormalForms Weakening GenericTyping Monad LogicalRelation DeclarativeInstance.
 From LogRel.LogicalRelation Require Import Induction Escape.
 
 Set Universe Polymorphism.
 
 Section Reflexivities.
   Context `{GenericTypingProperties}.
+  
+  Definition reflLRTyEq {l wl Γ A} (lr : [ Γ ||-< l > A ]< wl > ) : [ Γ ||-< l > A ≅ A | lr ]< wl >.
+  Proof.
+    pattern l, wl, Γ, A, lr; eapply LR_rect_TyUr; intros ???? [] **.
+    all: try match goal with H : PolyRed _ _ _ _ _ |- _ => destruct H; econstructor; tea end.
+    all: try now econstructor.
+    Unshelve.
+    all: cbn in * ; try eassumption.
+    (* econstructor; tea; now eapply escapeEqTerm. *)
+  Qed.
 
-  Definition LRTyEqRefl {l wl Γ A eqTy redTm eqTm}
+  (* Deprecated *)
+  Corollary LRTyEqRefl {l wl Γ A eqTy redTm eqTm}
     (lr : LogRel l wl Γ A eqTy redTm eqTm) : eqTy A.
   Proof.
-    induction lr as [ ? ? ? [] | ? ? ? [] | ? ? ? [] ? IHdom IHcod | ??? [] | ??? [] | ??? []].
-    all: try now unshelve econstructor.
-    cbn in *.
-    unshelve econstructor ; [exact dom | exact cod | .. ] ; try assumption ; cbn in *.
-    - intros.
-      now eapply (codomN Δ a l' ρ τ Ninfl h).
-    - intros ; eapply IHdom.
-    - intros ; now eapply IHcod.
+    pose (R := Build_LRPack wl Γ A eqTy redTm eqTm). 
+    pose (Rad := Build_LRAdequate (pack:=R) lr).
+    change [Rad | _ ||- _ ≅ A ]< _ >; now eapply reflLRTyEq.
   Qed.
 
-  Corollary LRTyEqRefl_ {l wl Γ A} (lr : [ Γ ||-< l > A ]< wl > ) : [ Γ ||-< l > A ≅ A | lr ]< wl >.
-  Proof.
-    destruct lr as [[] lr].
-    cbn in *.
-    now eapply LRTyEqRefl.
-  Qed.
-
-  Corollary WLRTyEqRefl_ {l wl Γ A} (lr : W[ Γ ||-< l > A ]< wl > ) : W[ Γ ||-< l > A ≅ A | lr ]< wl >.
-  Proof.
-    destruct lr.
-    exists WN.
-    intros.
-    eapply LRTyEqRefl_.
-  Qed.
-  
   Lemma NeNfEqRefl {wl Γ k A} : [Γ ||-NeNf k : A]< wl > -> [Γ ||-NeNf k ≅ k : A]< wl >.
   Proof.
     intros []; now econstructor.
   Qed.
 
   Lemma reflNatRedTmEq {wl Γ A} {NA : [Γ ||-Nat A]< wl >} :
-    (forall t : term, [Γ ||-Nat t : A | NA]< wl > ->
-                      [Γ ||-Nat t ≅ t : A | NA]< wl >)
+      (forall t : term, [Γ ||-Nat t : A | NA]< wl > -> [Γ ||-Nat t ≅ t : A | NA]< wl >)
     × (forall t : term, NatProp NA t -> NatPropEq NA t t).
   Proof.
     eapply NatRedInduction.
@@ -52,79 +42,85 @@ Section Reflexivities.
     intros; econstructor.
     now eapply NeNfEqRefl.
   Qed.
-  
-  Lemma reflBoolRedTmEq {wl Γ A} {NA : [Γ ||-Bool A]< wl >} :
-    (forall t : term, [Γ ||-Bool t : A | NA]< wl > ->
-                      [Γ ||-Bool t ≅ t : A | NA]< wl >)
-    × (forall t : term, BoolProp NA t -> BoolPropEq NA t t).
-  Proof.
-    split.
-    - intros t Ht ; induction Ht.
-      econstructor ; eauto.
-      destruct prop; econstructor.
-      now eapply NeNfEqRefl.
-    - intros ? [] ;  econstructor. 
-      now eapply NeNfEqRefl.
-  Qed.
 
-  Lemma reflEmptyRedTmEq {wl Γ A} {NA : [Γ ||-Empty A]< wl >} :
-      (forall t : term, [Γ ||-Empty t : A | NA]< wl > -> [Γ ||-Empty t ≅ t : A | NA]< wl >)
-    × (forall t : term, @EmptyProp _ _ _ _ wl Γ t -> @EmptyPropEq _ _ _ wl Γ t t).
+  Lemma reflBoolRedTmEq {wl Γ A} {NA : [Γ ||-Bool A]< wl >} :
+      (forall t : term, [Γ ||-Bool t : A | NA]< wl > -> [Γ ||-Bool t ≅ t : A | NA]< wl >)
+    × (forall t : term, BoolProp NA t -> BoolPropEq NA t t).
   Proof.
     split.
     - intros t Ht. induction Ht.
       econstructor; eauto.
       destruct prop; econstructor.
       now eapply NeNfEqRefl.
-    - intros ? []. econstructor. 
+    - intros ? [].
+      + econstructor.
+      + econstructor.
+      + econstructor.
+        now eapply NeNfEqRefl.
+  Qed.
+
+  Lemma reflEmptyRedTmEq {wl Γ A} {NA : [Γ ||-Empty A]< wl >} :
+      (forall t : term, [Γ ||-Empty t : A | NA]< wl > -> [Γ ||-Empty t ≅ t : A | NA]< wl >)
+    × (forall t : term, @EmptyProp _ _ _ wl Γ t -> @EmptyPropEq _ _ wl Γ t t).
+  Proof.
+    split.
+    - intros t Ht. induction Ht.
+      econstructor; eauto.
+      destruct prop; econstructor.
+      now eapply NeNfEqRefl.
+    - intros ? []. econstructor.
       now eapply NeNfEqRefl.
   Qed.
 
-  Definition LRTmEqRefl@{h i j k l} {l wl Γ A eqTy redTm eqTm} (lr : LogRel@{i j k l} l wl Γ A eqTy redTm eqTm) :
-    forall t, redTm t -> eqTm t t.
+  Lemma reflIdPropEq {wl Γ l A} (IA : [Γ ||-Id<l> A]< wl >) t (Pt : IdProp IA t) : IdPropEq IA t t.
   Proof.
-    induction lr as [ ? ? ? h | ? ? ? [] | ? ? ? [] IHdom IHcod| ??? NA | ??? NA | ??? NA].
-    - intros t [? ? ? ? ? [[] rel]%RedTyRecFwd] ; cbn in *.
+    destruct Pt; constructor; tea; now eapply NeNfEqRefl.
+  Qed.
+
+  Lemma reflIdRedTmEq {wl Γ l A} (IA : [Γ ||-Id<l> A]< wl >) t (Rt : [Γ ||-Id<l> t : _ | IA]< wl >) : [Γ ||-Id<l> t ≅ t : _ | IA]< wl >.
+  Proof. destruct Rt; econstructor; tea; now eapply reflIdPropEq. Qed.
+
+  Definition reflLRTmEq@{h i j k l} {l wl Γ A} (lr : [ LogRel@{i j k l} l | Γ ||- A ]< wl > ) :
+    forall t,
+      [ Γ ||-<l> t : A | lr ]< wl > ->
+      [ Γ ||-<l> t ≅ t : A | lr ]< wl >.
+  Proof.
+    pattern l, wl, Γ, A, lr; eapply LR_rect_TyUr; clear l wl Γ A lr; intros l wl Γ A.
+    - intros h t [? ? ? ? Rt%RedTyRecFwd@{j k h i k}] ; cbn in *.
       (* Need an additional universe level h < i *)
-      assert (eqTy t) by (eapply LRTyEqRefl@{h i j k}; exact rel).
+      Unset Printing Notations.
+      pose proof (reflLRTyEq@{h i k j} Rt).
       unshelve econstructor.
       all : cbn.
       1-2: econstructor ; tea ; cbn.
-      1-3,5: eapply RedTyRecBwd; apply (LRbuild@{h i j k} rel).
+      1-3,5: eapply RedTyRecBwd; tea.
       1: cbn; easy.
       now eapply TyEqRecBwd.
-    - intros t [].
+    - intros [] t [].
       econstructor ; cbn in *.
       all: eassumption.
-    - intros t [].
+    - intros ??? t [].
       unshelve econstructor ; cbn in *.
       1-2: now econstructor.
-      all: cbn.
-      all: now eauto.
-    - apply reflNatRedTmEq.
-    - apply reflBoolRedTmEq.
-    - apply reflEmptyRedTmEq. 
+      all: cbn; now eauto.
+    - intros; now apply reflNatRedTmEq.
+    - intros; now apply reflBoolRedTmEq.
+    - intros; now apply reflEmptyRedTmEq.
+    - intros ??? t [].
+      unshelve econstructor ; cbn in *.
+      1-2: now econstructor.
+      all: cbn; now eauto.
+    - intros; now eapply reflIdRedTmEq.
   Qed.
-
-  Definition LREqTermRefl_ {l wl Γ A t} (lr : [ Γ ||-< l > A ]< wl > ) : 
-      [ Γ ||-< l > t : A | lr ]< wl > ->
-      [ Γ ||-< l > t ≅ t : A | lr ]< wl >.
+  
+  (* Deprecated *)
+  Corollary LRTmEqRefl@{h i j k l} {l wl Γ A eqTy redTm eqTm} (lr : LogRel@{i j k l} l wl Γ A eqTy redTm eqTm) :
+    forall t, redTm t -> eqTm t t.
   Proof.
-    destruct lr as [[] lr].
-    cbn in *.
-    now eapply LRTmEqRefl.
+    pose (R := Build_LRPack wl Γ A eqTy redTm eqTm). 
+    pose (Rad := Build_LRAdequate (pack:=R) lr).
+    intros t ?; change [Rad | _ ||- t ≅ t : _ ]< _ >; now eapply reflLRTmEq.
   Qed.
-
-  Corollary WLREqTermRefl_ {l wl Γ A t} (lr : W[ Γ ||-< l > A ]< wl > ) : 
-      W[ Γ ||-< l > t : A | lr ]< wl > ->
-      W[ Γ ||-< l > t ≅ t : A | lr ]< wl >.
-  Proof.
-    intros [].
-    destruct lr.
-    exists WNTm.
-    intros.
-    eapply LREqTermRefl_.
-    now eapply WRedTm.
-  Qed.    
 
 End Reflexivities.
+
