theories/GenericTyping.v
@@ -668,9 +668,9 @@ Class GenericTypingProperties `(ta : tag)
 (* Priority 2 *)
 #[export] Hint Resolve wfc_nil wfc_cons | 2 : gen_typing.
 #[export] Hint Resolve wft_wk wft_U wft_prod wft_sig wft_Id | 2 : gen_typing.
-#[export] Hint Resolve ty_wk ty_var ty_prod ty_lam ty_app ty_nat ty_empty ty_zero ty_succ ty_natElim ty_emptyElim ty_sig ty_pair ty_fst ty_snd ty_Id ty_refl ty_IdElim| 2 : gen_typing.
+#[export] Hint Resolve ty_wk ty_var ty_prod ty_lam ty_app ty_nat ty_bool ty_empty ty_zero ty_succ ty_natElim ty_true ty_false ty_alpha ty_boolElim ty_emptyElim ty_sig ty_pair ty_fst ty_snd ty_Id ty_refl ty_IdElim| 2 : gen_typing.
 #[export] Hint Resolve convty_wk convty_uni convty_prod convty_sig convty_Id | 2 : gen_typing.
-#[export] Hint Resolve convtm_wk convtm_prod convtm_eta convtm_nat convtm_empty convtm_zero convtm_succ convtm_eta_sig convtm_Id convtm_refl | 2 : gen_typing.
+#[export] Hint Resolve convtm_wk convtm_prod convtm_eta convtm_nat convtm_bool convtm_empty convtm_zero convtm_succ convtm_true convtm_false convtm_alphacong convtm_eta_sig convtm_Id convtm_refl | 2 : gen_typing.
 #[export] Hint Resolve convneu_wk convneu_var convneu_app convneu_natElim convneu_emptyElim convneu_fst convneu_snd convneu_IdElim | 2 : gen_typing.
 #[export] Hint Resolve redty_ty_src redtm_ty_src | 2 : gen_typing.
 (* Priority 4 *)
@@ -840,7 +840,7 @@ Section GenericConsequences.
 
   #[local] Hint Resolve tyr_wf_l tmr_wf_l : gen_typing.
   #[local] Hint Resolve redty_wk redty_term redty_refl redtm_wk redtm_app redtm_refl | 2 : gen_typing.
-  #[local] Hint Resolve redtm_beta redtm_natElimZero redtm_natElimSucc | 2 : gen_typing.
+  #[local] Hint Resolve redtm_beta redtm_natElimZero redtm_natElimSucc redtm_boolElimTrue redtm_boolElimFalse | 2 : gen_typing.
   #[local] Hint Resolve  redtm_conv | 6 : gen_typing.
 
   Lemma redty_red {l Γ A B} :
@@ -950,6 +950,25 @@ Section GenericConsequences.
     intros ???; constructor; tea; gen_typing.
   Qed.
 
+  Lemma redtmwf_boolElimTrue {l Γ P ht hf} :
+    [Γ ,, tBool |- P ]< l > ->
+    [Γ |- ht : P[tTrue..]]< l > ->
+    [Γ |- hf : P[tFalse..]]< l > ->
+    [Γ |- tBoolElim P ht hf tTrue :⤳*: ht : P[tTrue..]]< l >.
+  Proof.
+    intros ???; constructor; tea; gen_typing.
+  Qed.
+
+  Lemma redtmwf_boolElimFalse {l Γ P ht hf} :
+    [Γ ,, tBool |- P ]< l > ->
+    [Γ |- ht : P[tTrue..]]< l > ->
+    [Γ |- hf : P[tFalse..]]< l > ->
+    [Γ |- tBoolElim P ht hf tFalse :⤳*: hf : P[tFalse..]]< l >.
+  Proof.
+    intros ???; constructor; tea; gen_typing.
+  Qed.
+
+  
   (** *** Properties of well-typing *)
 
   Definition well_typed_well_formed l Γ t : well_typed l Γ t -> well_formed l Γ t :=
@@ -1410,5 +1429,5 @@ Section GenericConsequences.
 End GenericConsequences.
 
 #[export] Hint Resolve tyr_wf_l tmr_wf_l well_typed_well_formed : gen_typing.
-#[export] Hint Resolve redtywf_wk redtywf_term redtywf_red redtywf_refl redtmwf_wk redtmwf_app redtmwf_refl redtm_beta redtmwf_red redtmwf_natElimZero | 2 : gen_typing.
+#[export] Hint Resolve redtywf_wk redtywf_term redtywf_red redtywf_refl redtmwf_wk redtmwf_app redtmwf_refl redtm_beta redtmwf_red redtmwf_natElimZero redtmwf_boolElimTrue redtmwf_boolElimFalse | 2 : gen_typing.
 #[export] Hint Resolve  redtmwf_conv | 6 : gen_typing.
