theories/LogicalRelation/Escape.v
@@ -1,8 +1,7 @@
 (** * LogRel.LogicalRelation.Escape: the logical relation implies conversion/typing. *)
-Require Import PeanoNat Nat.
 From Coq Require Import CRelationClasses.
 From LogRel.AutoSubst Require Import core unscoped Ast Extra.
-From LogRel Require Import Utils BasicAst Notations LContexts Context NormalForms GenericTyping LogicalRelation DeclarativeInstance.
+From LogRel Require Import Utils BasicAst Notations LContexts Context NormalForms GenericTyping Monad LogicalRelation.
 From LogRel.LogicalRelation Require Import Induction.
 
 Set Universe Polymorphism.
@@ -26,45 +25,27 @@ Section Escapes.
     - intros ???? []; gen_typing.
     - intros ???? []; gen_typing.
     - intros ???? []; gen_typing.
+    - intros ???? []; gen_typing.
+    - intros ???? []; gen_typing.
   Qed.
 
   Lemma Wescape {l wl Γ A} :
     W[ Γ ||-< l > A ]< wl > -> [Γ |- A]< wl >.
   Proof.
     intros [].
-    remember (Lack_n wl WN) as q.
-    revert wl Heqq WRed.
-    induction q ; intros.
+    revert WRed ; induction WT ; cbn ; intros.
     - eapply escape.
       eapply WRed.
-      + now eapply wfLCon_le_id.
-      + eapply Lack_nil_AllInLCon.
-        now symmetry.
-    - unshelve eapply wft_ϝ.
-      + exact a.
-      + unshelve eapply Lack_n_notinLCon.
-        exact WN.
-        rewrite <- Heqq.
-        cbn.
-        now left.
-      + eapply IHq.
-        * symmetry.
-          eapply Lack_n_add.
-          now symmetry.
-        * intros * f allinl.
-          eapply WRed ; try eassumption.
-          eapply wfLCon_le_trans ; try eassumption.
-          eapply LCon_le_step.
-          now eapply wfLCon_le_id.
-      + eapply IHq.
-        * symmetry.
-          eapply Lack_n_add.
-          now symmetry.
-        * intros * f allinl.
-          eapply WRed ; try eassumption.
-          eapply wfLCon_le_trans ; try eassumption.
-          eapply LCon_le_step.
-          now eapply wfLCon_le_id.
+      now eapply wfLCon_le_id.
+    - unshelve eapply (wft_ϝ (ne := ne)).
+      + eapply IHWT1.
+        intros wl' Hover ; eapply WRed.
+        assert (Hyp := over_tree_le Hover _ _ (in_here_l _)).
+        now erewrite (decidInLCon_true Hyp).
+      + eapply IHWT2.
+        intros wl' Hover ; eapply WRed.
+        assert (Hyp := over_tree_le Hover _ _ (in_here_l _)).
+        now erewrite (decidInLCon_false Hyp).
   Qed.
   
   Lemma escapeEq {l wl Γ A B} (lr : [Γ ||-< l > A]< wl >) :
@@ -83,6 +64,10 @@ Section Escapes.
     + intros ???? [] []; gen_typing.
     + intros ???? [] []; gen_typing.
     + intros ???? [] []; gen_typing.
+    + intros ???? [] * ? ? []; cbn in *.
+      eapply convty_exp. all: try gen_typing.
+    + intros ???? [???? red] ?? [???? red']; cbn in *. 
+      eapply convty_exp; tea;[eapply red | eapply red'].
   Qed.
 
   Lemma WescapeEq {l wl Γ A B} (lr : W[Γ ||-< l > A]< wl >) :
@@ -90,47 +75,31 @@ Section Escapes.
       [Γ |- A ≅ B]< wl >.
   Proof.
     intros [].
-    destruct lr as [WN WRed].
-    remember (Lack_n wl (max WN WNEq)) as q.
-    revert wl Heqq WRed WRedEq.
-    induction q ; intros.
+    destruct lr as [WT WRed] ; cbn in *.
+    pose (d := DTree_fusion _ WT WTEq).
+    assert ({dWRed : forall wl' : wfLCon, over_tree wl wl' d -> [Γ ||-< l > A ]< wl' > &
+              forall (wl' : wfLCon) (Hover : over_tree wl wl' d), [dWRed wl' Hover | _ ||- _ ≅ B ]< _ >}) as [dWRed dWRedEq].
+    { exists (fun wl' Hover => WRed wl' (over_tree_fusion_l Hover)).
+      intros wl' Hover ; cbn. eapply WRedEq.
+      eapply over_tree_fusion_r. eassumption.
+    }
+    revert dWRed dWRedEq ; generalize d ; clear d WT WRed WTEq WRedEq.
+    intros d.
+    induction d as [ | wl' n ne ? IHEqt ? IHEqf] ; cbn ; intros.
     - unshelve eapply escapeEq ; [assumption | ..].
-      1: eapply WRed ; [now eapply wfLCon_le_id | ..].
-      2: eapply WRedEq.
-      all: eapply Lack_nil_AllInLCon ;
-        eapply Incl_nil ;
-        rewrite Heqq ;
-        eapply Lack_n_le.
-      1: now eapply Nat.le_max_l.
-      now eapply Nat.le_max_r.
-    - unshelve eapply convty_ϝ.
-      + exact a.
-      + unshelve eapply Lack_n_notinLCon.
-        exact (max WN WNEq).
-        rewrite <- Heqq.
-        now left.
-      + unshelve eapply IHq.
-        * intros * allinl.
-          eapply WRed ; try eassumption.
-          eapply wfLCon_le_trans ; try eassumption.
-          eapply LCon_le_step.
-          now eapply wfLCon_le_id.
-        * symmetry.
-          eapply Lack_n_add.
-          now symmetry.
-        * intros * allinl.
-          now eapply WRedEq ; try eassumption.
-      + unshelve eapply IHq.
-        * intros * allinl.
-          eapply WRed ; try eassumption.
-          eapply wfLCon_le_trans ; try eassumption.
-          eapply LCon_le_step.
-          now eapply wfLCon_le_id.
-        * symmetry.
-          eapply Lack_n_add.
-          now symmetry.
-        * intros * allinl.
-          now eapply WRedEq ; try eassumption.
+      1: eapply dWRed.
+      2: eapply dWRedEq.
+      all: now apply wfLCon_le_id.
+    - unshelve eapply (convty_ϝ (ne := ne)).
+      + eapply IHEqt.
+        intros wl'' Hover ; eapply dWRedEq.
+        Unshelve.
+        assert (Hyp := over_tree_le Hover _ _ (in_here_l _)).
+        now erewrite (decidInLCon_true Hyp).
+      + eapply IHEqf.
+        intros wl'' Hover ; unshelve eapply dWRedEq.
+        assert (Hyp := over_tree_le Hover _ _ (in_here_l _)).
+        now erewrite (decidInLCon_false Hyp).
   Qed.
   
   Definition escapeTerm {l wl Γ t A} (lr : [Γ ||-< l > A ]< wl >) :
@@ -147,6 +116,10 @@ Section Escapes.
     - intros ???? [] []; gen_typing.
     - intros ???? [] []; gen_typing.
     - intros ???? [] []; gen_typing.
+    - intros ???? [] * ?? [] ; cbn in *.
+      gen_typing.
+    - intros ???? IA _ _ []. 
+      unfold_id_outTy; destruct IA; cbn in *; gen_typing.
   Qed.
 
   Definition WescapeTerm {l wl Γ t A} (lr : W[Γ ||-< l > A ]< wl >) :
@@ -154,47 +127,31 @@ Section Escapes.
     [Γ |- t : A]< wl >.
   Proof.
     intros [].
-    destruct lr as [WN WRed].
-    remember (Lack_n wl (max WN WNTm)) as q.
-    revert wl Heqq WRed WRedTm.
-    induction q ; intros.
+    destruct lr as [WT WRed].
+    pose (d := DTree_fusion _ WT WTTm).
+    assert ({dWRed : forall wl' : wfLCon, over_tree wl wl' d -> [Γ ||-< l > A ]< wl' > &
+                      forall (wl' : wfLCon) (Hover : over_tree wl wl' d), [dWRed wl' Hover | _ ||- t : _ ]< _ >})
+      as [dWRed dWRedTm].
+    { exists (fun wl' Hover => WRed wl' (over_tree_fusion_l Hover)).
+      intros wl' Hover ; cbn. eapply WRedTm.
+      eapply over_tree_fusion_r. eassumption.
+    }
+    revert dWRed dWRedTm ; generalize d ; clear d WT WRed WTTm WRedTm.
+    intros d.
+    induction d as [ | wl' n ne ? IHEqt ? IHEqf] ; cbn ; intros.
     - unshelve eapply escapeTerm ; [assumption | ..].
-      1: eapply WRed ; [now eapply wfLCon_le_id | ..].
-      2: eapply WRedTm.
-      all: eapply Lack_nil_AllInLCon ;
-        eapply Incl_nil ;
-        rewrite Heqq ;
-        eapply Lack_n_le.
-      1: now eapply Nat.le_max_l.
-      now eapply Nat.le_max_r.
-    - unshelve eapply ty_ϝ.
-      + exact a.
-      + unshelve eapply Lack_n_notinLCon.
-        exact (max WN WNTm).
-        rewrite <- Heqq.
-        now left.
-      + unshelve eapply IHq.
-        * intros * f allinl.
-          eapply WRed ; try eassumption.
-          eapply wfLCon_le_trans ; try eassumption.
-          eapply LCon_le_step.
-          now eapply wfLCon_le_id.
-        * symmetry.
-          eapply Lack_n_add.
-          now symmetry.
-        * intros * allinl.
-          now eapply WRedTm ; try eassumption.
-      + unshelve eapply IHq.
-        * intros * f allinl.
-          eapply WRed ; try eassumption.
-          eapply wfLCon_le_trans ; try eassumption.
-          eapply LCon_le_step.
-          now eapply wfLCon_le_id.
-        * symmetry.
-          eapply Lack_n_add.
-          now symmetry.
-        * intros * allinl.
-          now eapply WRedTm ; try eassumption.
+      1: eapply dWRed ; [now eapply wfLCon_le_id | ..].
+      now eapply dWRedTm.
+    - unshelve eapply (ty_ϝ (ne := ne)).
+      + eapply IHEqt.
+        intros wl'' Hover ; eapply dWRedTm.
+        Unshelve.
+        assert (Hyp := over_tree_le Hover _ _ (in_here_l _)).
+        now erewrite (decidInLCon_true Hyp).
+      + eapply IHEqf.
+        intros wl'' Hover ; unshelve eapply dWRedTm.
+        assert (Hyp := over_tree_le Hover _ _ (in_here_l _)).
+        now erewrite (decidInLCon_false Hyp).
   Qed.
    
   Definition escapeEqTerm {l wl Γ t u A} (lr : [Γ ||-< l > A ]< wl >) :
@@ -203,19 +160,37 @@ Section Escapes.
   Proof.
     pattern l, wl, Γ, A, lr ; eapply LR_rect_TyUr.
     - intros ???? [] [[] []] ; cbn in *.
+      eapply (convtm_conv (A := U)).
       eapply convtm_exp ; tea.
       all: gen_typing.
-    - intros ???? [] [] ; cbn in *.
+    - intros ???? [ty] [] ; cbn in *.
+      assert (isPosType ty).
+      {
+      constructor.
+      now eapply convneu_whne. 
+      }
+      eapply (convtm_conv (A := ty)).
       eapply convtm_exp ; tea.
       all: gen_typing.
-    - intros ???? [] * ?? [[termL] [termR]] ; cbn in *.
+    - intros ???? [dom cod] * ?? [[termL] [termR]] ; cbn in *.
+      eapply (convtm_conv (A := tProd dom cod)).
       eapply convtm_exp ; tea.
       all: gen_typing.
     - intros ???? [] []; cbn in *.
+      eapply (convtm_conv (A := tNat)); [|gen_typing].
       eapply convtm_exp; tea; gen_typing.
     - intros ???? [] []; cbn in *.
+      eapply (convtm_conv (A := tBool)); [|gen_typing].
       eapply convtm_exp; tea; gen_typing.
     - intros ???? [] []; cbn in *.
+      eapply (convtm_conv (A := tEmpty)); [|gen_typing].
+      eapply convtm_exp; tea; gen_typing.
+    - intros ???? [dom cod] * ?? [[termL] [termR]] ; cbn in *.
+      eapply (convtm_conv (A := tSig dom cod)).
+      eapply convtm_exp ; tea.
+      all: gen_typing.
+    - intros ???? [ty lhs rhs] _ _ []; unfold_id_outTy; cbn in *.
+      eapply (convtm_conv (A := tId ty lhs rhs)); [|gen_typing].
       eapply convtm_exp; tea; gen_typing.
   Qed.
 
@@ -224,47 +199,30 @@ Section Escapes.
     [Γ |- t ≅ u : A]< wl >.
   Proof.
     intros [].
-    destruct lr as [WN WRed].
-    remember (Lack_n wl (max WN WNTmEq)) as q.
-    revert wl Heqq WRed WRedTmEq.
-    induction q ; intros.
-    - unshelve eapply escapeEqTerm ; [assumption | ..].
-      1: eapply WRed ; [now eapply wfLCon_le_id | ..].
-      2: eapply WRedTmEq.
-      all: eapply Lack_nil_AllInLCon ;
-        eapply Incl_nil ;
-        rewrite Heqq ;
-        eapply Lack_n_le.
-      1: now eapply Nat.le_max_l.
-      now eapply Nat.le_max_r.
-    - unshelve eapply convtm_ϝ.
-      + exact a.
-      + unshelve eapply Lack_n_notinLCon.
-        exact (max WN WNTmEq).
-        rewrite <- Heqq.
-        now left.
-      + unshelve eapply IHq.
-        * intros * allinl.
-          eapply WRed ; try eassumption.
-          eapply wfLCon_le_trans ; try eassumption.
-          eapply LCon_le_step.
-          now eapply wfLCon_le_id.
-        * symmetry.
-          eapply Lack_n_add.
-          now symmetry.
-        * intros * allinl.
-          now eapply WRedTmEq ; try eassumption.
-      + unshelve eapply IHq.
-        * intros * allinl.
-          eapply WRed ; try eassumption.
-          eapply wfLCon_le_trans ; try eassumption.
-          eapply LCon_le_step.
-          now eapply wfLCon_le_id.
-        * symmetry.
-          eapply Lack_n_add.
-          now symmetry.
-        * intros * allinl.
-          now eapply WRedTmEq ; try eassumption.
+    destruct lr as [WT WRed].
+    pose (d := DTree_fusion _ WT WTTmEq).
+    assert ({H : forall wl' : wfLCon, over_tree wl wl' d -> [Γ ||-< l > A ]< wl' > &
+                   forall (wl' : wfLCon) (Hover : over_tree wl wl' d), [H wl' Hover | _ ||- t  ≅ u : _ ]< _ >})
+      as [dWRed dWRedTmEq].
+    { exists (fun wl' Hover => WRed wl' (over_tree_fusion_l Hover)).
+      intros wl' Hover ; cbn ; eapply WRedTmEq.
+      eapply over_tree_fusion_r ; eassumption.
+    }
+    revert dWRed dWRedTmEq ; generalize d ; clear d WT WRed WTTmEq WRedTmEq.
+    intros d.
+    induction d as [ | wl' n ne ? IHEqt ? IHEqf] ; cbn ; intros.
+    - eapply escapeEqTerm.
+      unshelve eapply dWRedTmEq.
+      now eapply wfLCon_le_id.
+    - unshelve eapply (convtm_ϝ (ne := ne)).
+      + eapply IHEqt.
+        intros wl'' Hover ; unshelve eapply dWRedTmEq.
+        assert (Hyp := over_tree_le Hover _ _ (in_here_l _)).
+        now erewrite (decidInLCon_true Hyp).
+      + eapply IHEqf.
+        intros wl'' Hover ; unshelve eapply dWRedTmEq.
+        assert (Hyp := over_tree_le Hover _ _ (in_here_l _)).
+        now erewrite (decidInLCon_false Hyp).
   Qed.
   
   
@@ -280,6 +238,8 @@ Section Escapes.
     - intros * []; gen_typing.
     - intros * []; gen_typing.
     - intros * []; gen_typing.
+    - intros * ??? []; gen_typing.
+    - intros * _ _ ? []; gen_typing.
   Qed.
 
   Lemma WescapeConv {l wl Γ A} (RA : W[Γ ||-<l> A]< wl >) :
@@ -288,47 +248,30 @@ Section Escapes.
     [Γ |- B]< wl >.
   Proof.
     intros B [].
-    destruct RA as [WN WRed].
-    remember (Lack_n wl (max WN WNEq)) as q.
-    revert wl Heqq WRed WRedEq.
-    induction q ; intros.
-    - unshelve eapply escapeConv ; [assumption | exact A | ..].
-      1: eapply WRed ; [now eapply wfLCon_le_id | ..].
-      2: eapply WRedEq.
-      all: eapply Lack_nil_AllInLCon ;
-        eapply Incl_nil ;
-        rewrite Heqq ;
-        eapply Lack_n_le.
-      1: now eapply Nat.le_max_l.
-      now eapply Nat.le_max_r.
-    - unshelve eapply wft_ϝ.
-      + exact a.
-      + unshelve eapply Lack_n_notinLCon.
-        exact (max WN WNEq).
-        rewrite <- Heqq.
-        now left.
-      + unshelve eapply IHq.
-        * intros * allinl.
-          eapply WRed ; try eassumption.
-          eapply wfLCon_le_trans ; try eassumption.
-          eapply LCon_le_step.
-          now eapply wfLCon_le_id.
-        * symmetry.
-          eapply Lack_n_add.
-          now symmetry.
-        * intros * allinl.
-          now eapply WRedEq ; try eassumption.
-      + unshelve eapply IHq.
-        * intros * allinl.
-          eapply WRed ; try eassumption.
-          eapply wfLCon_le_trans ; try eassumption.
-          eapply LCon_le_step.
-          now eapply wfLCon_le_id.
-        * symmetry.
-          eapply Lack_n_add.
-          now symmetry.
-        * intros * allinl.
-          now eapply WRedEq ; try eassumption.
+    destruct RA as [WT WRed].
+    pose (d := DTree_fusion _ WT WTEq) ; cbn in *.
+    assert ({H : forall wl' : wfLCon, over_tree wl wl' d -> [Γ ||-< l > A ]< wl' > &
+                   forall (wl' : wfLCon) (Hover : over_tree wl wl' d), [H wl' Hover | _ ||- _ ≅ B ]< _ >})
+      as [dWRed dWRedEq].
+    { exists (fun wl' Hover => WRed wl' (over_tree_fusion_l Hover)).
+      intros wl' Hover ; cbn ; eapply WRedEq.
+      eapply over_tree_fusion_r ; eassumption.
+    }
+    revert dWRed dWRedEq ; generalize d ; clear d WT WRed WTEq WRedEq.
+    intros d.
+    induction d as [ | wl' n ne ? IHEqt ? IHEqf] ; cbn ; intros.
+    - eapply escapeConv.
+      unshelve eapply dWRedEq.
+      now eapply wfLCon_le_id.
+    - unshelve eapply (wft_ϝ (ne := ne)).
+      + eapply IHEqt.
+        intros wl'' Hover ; unshelve eapply dWRedEq.
+        assert (Hyp := over_tree_le Hover _ _ (in_here_l _)).
+        now erewrite (decidInLCon_true Hyp).
+      + eapply IHEqf.
+        intros wl'' Hover ; unshelve eapply dWRedEq.
+        assert (Hyp := over_tree_le Hover _ _ (in_here_l _)).
+        now erewrite (decidInLCon_false Hyp).
   Qed.
   
 End Escapes.
