theories/LogicalRelation/ShapeView.v
@@ -23,6 +23,8 @@ Section ShapeViews.
       | LRNat _ _, LRNat _ _ => True
       | LRBool _ _, LRBool _ _ => True
       | LREmpty _ _, LREmpty _ _ => True
+      | LRSig _ _ _, LRSig _ _ _ => True
+      | LRId _ _ _, LRId _ _ _ => True
       | _, _ => False
     end.
 
@@ -42,19 +44,22 @@ when showing symmetry or transitivity of the logical relation. *)
 
   Lemma red_whnf@{i j k l} {wl Γ A lA eqTyA redTmA eqTmA}
     (lrA : LogRel@{i j k l} lA wl Γ A eqTyA redTmA eqTmA) : 
-    ∑ nf, [Γ |- A :⇒*: nf]< wl > × whnf nf.
+    ∑ nf, [Γ |- A :⤳*: nf]< wl > × whnf nf.
   Proof.
-    destruct lrA as [??? []| ??? [] | ??? []| ??? [] | ??? [] | ??? []];
-      eexists; split; tea; constructor; tea.
-    now eapply ty_ne_whne.
+    pattern lA, wl, Γ, A, eqTyA, redTmA, eqTmA, lrA; eapply LR_rect; intros ???[].
+    all: eexists; split; tea; constructor; tea.
+    now eapply convneu_whne.
   Defined.
 
   Lemma eqTy_red_whnf@{i j k l} {wl Γ A lA eqTyA redTmA eqTmA B}
     (lrA : LogRel@{i j k l} lA wl Γ A eqTyA redTmA eqTmA) : 
-    eqTyA B -> ∑ nf, [Γ |- B :⇒*: nf]< wl > × whnf nf.
+    eqTyA B -> ∑ nf, [Γ |- B :⤳*: nf]< wl > × whnf nf.
   Proof.
-    destruct lrA as [??? []| ???[] | ???[]| ???[] | ???[] | ???[]] ; intros []; eexists; split; tea; constructor; tea.
-    now eapply ty_ne_whne.
+    pattern lA, wl, Γ, A, eqTyA, redTmA, eqTmA, lrA.
+    eapply LR_rect_LogRelRec@{i j k l k}; intros ???? [].
+    3,7,8: intros ??.
+    all: intros []; eexists; split; tea; constructor; tea.
+    eapply convneu_whne; now symmetry.
   Defined.
 
 
@@ -66,11 +71,11 @@ when showing symmetry or transitivity of the logical relation. *)
     intros eqAB.
     pose (x := eqTy_red_whnf lrA eqAB).
     pose (y:= red_whnf lrB).
-    pose proof (h := redtywf_det _ _ _ _ _ (snd x.π2) (snd y.π2) (fst x.π2) (fst y.π2)).
+    pose proof (h := redtywf_det (snd x.π2) (snd y.π2) (fst x.π2) (fst y.π2)).
     revert eqAB x y h. 
     destruct lrA; destruct lrB; intros []; cbn; try easy; try discriminate.
-    all: try now (intros e; rewrite e in ne; apply ty_ne_whne in ne; inversion ne).
-    all: try now (intros e; destruct neA as [? ? ne]; rewrite <- e in ne; apply ty_ne_whne in ne; inversion ne).
+    all: try now (intros e; destruct neA as [? ? ne]; subst; apply convneu_whne in ne; inversion ne).
+    all: try now (intros e; subst; symmetry in eq; apply convneu_whne in eq; inversion eq).
   Qed.
 
 (** ** More properties *)
@@ -98,6 +103,8 @@ when showing symmetry or transitivity of the logical relation. *)
       | LRNat _ _, LRNat _ _, LRNat _ _ => True
       | LRBool _ _, LRBool _ _, LRBool _ _ => True
       | LREmpty _ _, LREmpty _ _, LREmpty _ _ => True
+      | LRSig _ _ _, LRSig _ _ _, LRSig _ _ _ => True
+      | LRId _ _ _, LRId _ _ _, LRId _ _ _ => True
       | _, _, _ => False
     end.
 
